Should now be able to use EVAL to evaluate US_SEM.

examples/Sugar2/official-semantics/UnclockedSemanticsScript.sml
@@ -48,6 +48,11 @@ val _ = intLib.deprecate_int();
 val _ = new_theory "UnclockedSemantics";
 
 (******************************************************************************
+* pureDefine doesn't export definitions to theCompset (for EVAL).
+******************************************************************************)
+val pureDefine = with_flag (computeLib.auto_import_definitions, false) Define;
+
+(******************************************************************************
 * B_SEM l b means "l |= b" where l is a letter, i.e. l : 'prop -> bool
 ******************************************************************************)
 val B_SEM_def =
@@ -81,7 +86,7 @@ val B_SEM =
 * where w is a word, i.e. a list of letters: w : ('prop -> bool)list
 ******************************************************************************)
 val US_SEM_def =
- Define
+ pureDefine
   `(US_SEM w (S_BOOL b) = (LENGTH w = 1) /\ B_SEM (ELEM w 0) b)
    /\
    (US_SEM w (S_CAT(r1,r2)) = 
